examples/seplogic/Lang.fst
@@ -1,7 +1,7 @@
 module Lang
 
-open FStar.ST
-open FStar.Heap
+open FStar.SL.ST
+open FStar.SL.Heap
 
 type t = UInt64.t
 type addr = ref t
@@ -20,46 +20,39 @@ let rec wpsep_command (#a:Type0) (c:command a) :st_wp a
 
     | Bind #a #b c1 c2 ->
       FStar.Classical.forall_intro (FStar.WellFounded.axiom1 #a #(command b) c2);
-      fun p h3 -> exists (h2':heap) (h2'':heap). disjoint h2' h2'' /\ h3 == h2' `join` h2'' /\
-     (wpsep_command c1) (fun x h1 -> exists (h1':heap) (h1'':heap). disjoint h1' h1'' /\ disjoint h1 h2'' /\ (h1 `join` h2'') == (h1' `join` h1'') /\
-     (wpsep_command (c2 x)) (fun y h2 -> disjoint h2 h1'' /\ p y (h2 `join` h1'')) h1') h2'
+      fun p h3 -> exists (h2':heap) (h2'':heap). h3 == join_tot h2' h2'' /\
+     (wpsep_command c1) (fun x h1 -> exists (h1':heap) (h1'':heap). (join_tot h1 h2'') == (join_tot h1' h1'') /\
+     (wpsep_command (c2 x)) (fun y h2 -> p y (join_tot h2 h1'')) h1') h2'
 
     | Read r ->
-      fun p h0 -> (exists (x:t). h0 == (r `points_to` x)) /\ (forall (x:t). h0 == (r `points_to` x) ==> p x h0)
+      fun p h0 -> (exists (x:t). h0 == (points_to r x)) /\ (forall (x:t). h0 == (points_to r x) ==> p x h0)
 
     | Write r y ->
-      fun p h0 -> (exists (x:t). h0 == (r `points_to` x)) /\ (forall (h1:heap). h1 == (r `points_to` y) ==> p () h1)
+      fun p h0 -> (exists (x:t). h0 == (points_to r x)) /\ (forall (h1:heap). h1 == (points_to r y) ==> p () h1)
 
     | Alloc ->
-      fun p h0 -> (h0 == emp) /\ (forall (r:addr) (h1:heap). (h1 == r `points_to` 0uL) ==> p r h1)
+      fun p h0 -> (h0 == emp) /\ (forall (r:addr) (h1:heap). (h1 == points_to r 0uL) ==> p r h1)
 
 let lift_wpsep (#a:Type0) (wp_sep:st_wp a) :st_wp a
-  = fun p h0 -> exists (h0':heap) (h0'':heap). disjoint h0' h0'' /\ h0 == (h0' `join` h0'') /\
-                                       wp_sep (fun x h1' -> disjoint h1' h0'' /\ p x (h1' `join` h0'')) h0'
+  = fun p h0 -> exists (h0':heap) (h0'':heap). h0 == (join_tot h0' h0'') /\ wp_sep (fun x h1' -> p x (join_tot h1' h0'')) h0'
 
-let lemma_read_write (phi:heap -> heap -> prop) (r:addr) (h:heap) (p1:squash (h `contains` r))
-  :Lemma (requires phi (h `restrict` r) (h `minus` r))
-         (ensures (exists (h':heap) (h'':heap). disjoint h' h'' /\ h == h' `join` h'' /\
-	                                  ((exists x. h' == (r `points_to` x)) /\ phi h' h'')))
+let lemma_read_write (phi:heap -> heap -> prop) (r:addr) (h:heap{h `contains` r })
+  :Lemma (requires phi (restrict h r) (minus h r))
+         (ensures (exists (h':heap) (h'':heap). (h == join_tot h' h'') /\ 
+	          ((exists x. h' == (points_to r x)) /\ phi h' h'')))
   = ()
 
 let lemma_alloc_return (phi:heap -> heap -> prop) (h:heap)
   :Lemma (requires (phi emp h))
-         (ensures (exists (h':heap) (h'':heap). disjoint h' h'' /\ h == h' `join` h'' /\ ((h' == emp) /\ phi h' h'')))
+         (ensures (exists (h':heap) (h'':heap). h == join_tot h' h'' /\ ((h' == emp) /\ phi h' h'')))
   = ()
 
 let lemma_bind (phi:heap -> heap -> heap -> heap -> prop) (h:heap)
-  :Lemma (requires (exists (h2':heap) (h2'':heap). disjoint h2' h2'' /\ h == h2' `join` h2'' /\
+  :Lemma (requires (exists (h2':heap) (h2'':heap). h == join_tot h2' h2'' /\
                                               phi h emp h2' h2''))
-         (ensures (exists (h1':heap) (h1'':heap). disjoint h1' h1'' /\ h == h1' `join` h1'' /\
-	          (exists (h2':heap) (h2'':heap). disjoint h2' h2'' /\ h1' == h2' `join` h2'' /\
+         (ensures (exists (h1':heap) (h1'':heap). h == join_tot h1' h1'' /\
+	          (exists (h2':heap) (h2'':heap). h1' == join_tot h2' h2'' /\
 		                             phi h1' h1'' h2' h2'')))
-  = ()
-
-let lemma_extract_disjoint 
-  (phi:heap -> heap -> heap -> heap ->  prop) (h2':heap) (h2'':heap) (p1:squash (disjoint h2' h2''))
-  :Lemma (requires (exists (h1':heap) (h1'':heap). disjoint h1' h1'' /\ join h2' h2'' == join h1' h1'' /\ phi h1' h1'' h2' h2''))
-         (ensures (exists (h1':heap) (h1'':heap). disjoint h1' h1'' /\ disjoint h2' h2'' /\ join h2' h2'' == join h1' h1'' /\ phi h1' h1'' h2' h2''))
   = ()
 
 let lemma_eq_implies_intro (phi:heap -> prop) (x:heap)
