examples/seplogic/Test.fst
@@ -2,11 +2,11 @@ module Test
 
 open Lang
 
-open FStar.Heap
+open FStar.SL.Heap
 
 open FStar.Tactics
 
-#reset-options "--log_queries --using_facts_from '* -FStar.Tactics -FStar.Reflection'"
+#reset-options "--using_facts_from '* -FStar.Tactics -FStar.Reflection'"
 
 let unfold_fns :list string = [
   "wp_command";
@@ -55,25 +55,23 @@ let rec split_all () :Tac unit =
 
 let simplify_contains_aux :tactic unit =
   or_else assumption''
-          ((apply_lemma (quote lemma_contains_r_join_restrict_minus);; norm []) `or_else`
-	   (apply_lemma (quote lemma_contains_join_h_emp);; norm [])            `or_else`
-	   (apply_lemma (quote lemma_contains_r_join_points_to_minus);; norm []))
+          ((apply_lemma (quote lemma_contains_r_join_tot_restrict_minus);; norm [])   `or_else`
+	   (apply_lemma (quote lemma_contains_r_join_tot_points_to_minus);; norm [])  `or_else`
+	   (apply_lemma (quote lemma_contains_r1_join_tot_restrict_minus);; norm [])  `or_else`
+	   (apply_lemma (quote lemma_contains_r1_join_tot_points_to_minus);; norm []) `or_else`
+           (apply_lemma (quote lemma_contains_join_tot_h_emp);; norm []))
 
 let simplify_contains :tactic unit =
   repeat simplify_contains_aux;;
   return ()
 
-let simplify_disjoint :tactic unit =
-  norm [];;
-  (apply_lemma (quote lemma_disjoint_restrict_minus);; norm [])  `or_else`
-  (apply_lemma (quote lemma_disjoint_points_to_minus);; norm []) `or_else`
-  (apply_lemma (quote lemma_emp_disjoint);; norm []);;
-  simplify_contains
-
 let simplify_restrict_aux :tactic unit =
   (apply_lemma (quote lemma_eq_l_cong);; norm []);;
-  (apply_lemma (quote lemma_restrict_join_h_emp);; norm []) `or_else`
-  (apply_lemma (quote lemma_restrict_r_join_points_to_minus);; norm []);;
+  (apply_lemma (quote lemma_restrict_r_join_tot_points_to_minus);; norm [])  `or_else`
+  (apply_lemma (quote lemma_restrict_r_join_tot_restrict_minus);; norm [])   `or_else`
+  (apply_lemma (quote lemma_restrict_r1_join_tot_restrict_minus);; norm [])  `or_else`
+  (apply_lemma (quote lemma_restrict_r1_join_tot_points_to_minus);; norm []) `or_else`
+  (apply_lemma (quote lemma_restrict_join_tot_h_emp);; norm []);;
   simplify_contains
 
 let simplify_restrict :tactic unit =
@@ -82,41 +80,92 @@ let simplify_restrict :tactic unit =
   return ()
 
 let step_bind :tactic unit = 
+  dump "In step_bind";;
   apply_lemma (quote lemma_bind);;
   norm []
 
 let step_read_write :tactic unit = 
-  apply_lemma (quote lemma_read_write);; 
+  dump "In step_read_write";;
+  apply_lemma (quote lemma_read_write);;
+  dump "A";;
   norm [];;
   simplify_contains
 
-let step_extract_disjoint :tactic unit =
-  apply_lemma (quote lemma_extract_disjoint);;
+let step_alloc_return :tactic unit =
+  dump "In step_alloc_return";;
+  apply_lemma (quote lemma_alloc_return);;
   norm [];;
-  simplify_disjoint
+  simplify_contains
 
 let step_eq_implies_intro :tactic unit =
   dump "In step_eq_implies_intro";;
   apply_lemma (quote lemma_eq_implies_intro);;
-  dump "After lemma_eq_implies_intro";;
   norm [];;
-  dump "After norm";;
-  g <-- cur_goal;
-  print (formula_to_string (term_as_formula g));;
-  split;;
-  dump "After split";;
-  print "After split";;
-  g <-- cur_goal;
-  print (formula_to_string (term_as_formula g));;
-  simplify_disjoint;;
-  dump "After simplify_disjoint"
+  dump "A"
+
+let step_eq_implies_intro' :tactic unit =
+  dump "In step_eq_implies_intro'";;
+  forall_intro;;
+  apply_lemma (quote lemma_eq_implies_intro);;
+  norm [];;
+  dump "B"
 
 let step_intro :tactic unit =
+  dump "In step_intro";;
   norm [];;
   forall_intro;;
   simplify_restrict;;
   implies_intro;;
   return ()
+
+let step :tactic unit =
+  dump "step";;
+  step_bind              `or_else`
+  step_read_write        `or_else`
+  step_alloc_return      `or_else`
+  step_eq_implies_intro  `or_else`
+  step_eq_implies_intro' `or_else`
+  step_intro             `or_else`
+  fail "step: failed"
+
+let simplify_select :tactic unit =
+ (apply_lemma (quote lemma_sel_r_join_tot_restrict_minus);; norm [])   `or_else`
+ (apply_lemma (quote lemma_sel_r_join_tot_points_to_minus);; norm [])  `or_else`
+ (apply_lemma (quote lemma_sel_r1_join_tot_restrict_minus);; norm [])  `or_else`
+ (apply_lemma (quote lemma_sel_r1_join_tot_points_to_minus);; norm []) `or_else`
+ (apply_lemma (quote lemma_sel_join_tot_h_emp);; norm [])              `or_else`
+ (apply_lemma (quote lemma_sel_join_tot_emp_h);; norm [])
+ 
+let step_select :tactic unit =
+ apply_lemma (quote lemma_eq_cong);; 
+ norm [];;
+ simplify_select;;
+ trytac trefl;;
+ return ()
+
+let rec repeat_step_select () :Tac unit =
+  (g <-- trytac cur_goal;
+  begin match g with
+  | None -> return ()
+  | Some _ -> repeat step_select;;
+              dump "After repeat simplify_sel";;
+              trytac ((trefl;; qed) `or_else` smt);;
+              repeat_step_select
+  end
+  ) ()
+
+let simplify :tactic unit =
+ split_all;;
+ repeat_step_select;;
+ return ()
+
+let solve :tactic unit =
+ norm [delta; delta_only unfold_steps; primops];;
+ trytac implies_intros';;
+ dump "Initial goal";;
+ repeat step;;
+ simplify;;
+ dump "End"
 
 (***** Examples *****)
 open FStar.UInt
@@ -124,29 +173,46 @@ open FStar.UInt64
 
 type t = UInt64.t
 
+let write_ok (h:heap) (r:addr) (n:t) =
+  let c = (Write r n) in
+  let p = fun _ h -> sel h r == n in
+  let post = (lift_wpsep (wpsep_command c)) p h in
+  assert_by_tactic (h `contains` r ==> post) solve
+
+let increment_ok (h:heap) (r:addr) (n:t) =
+  let c = Bind (Read r) (fun n -> Write r (n +?^ 1uL)) in
+  let p = fun _ h -> (sel h r == n +?^ 1uL) in
+  let post = (lift_wpsep (wpsep_command c)) p h in
+  assert_by_tactic (h `contains` r /\ sel h r == n ==> post) solve
+
+let swap_ok (r1:addr) (r2:addr) (h:heap) (a:t) (b:t) =
+  let c = Bind (Read r1) (fun n1 -> Bind (Read r2) (fun n2 -> Bind (Write r1 n2) (fun _ -> Write r2 n1))) in
+  let p = fun _ h -> (sel h r1 == b /\ sel h r2 == a) in
+  let post = (lift_wpsep (wpsep_command c)) p h in
+  assert_by_tactic (h `contains` r1 /\  h `contains` r2 /\ addr_of r1 <> addr_of r2 /\ sel h r1 == a /\ sel h r2 == b ==> post) solve
 
 let double_increment_ok (r:addr) (h:heap) (n:t{size (v n + 2) FStar.UInt64.n}) =
   let c = Bind (Bind (Read r) (fun y -> Write r (y +?^ 1uL))) (fun _ -> (Bind (Read r) (fun y -> Write r (y +?^ 1uL))))  in
   let p = fun _ h -> sel h r == (n +?^ 2uL) in
   let t = (lift_wpsep (wpsep_command c)) p h in
-  assert_by_tactic (h `contains` r /\ sel h r == n ==> t) (
-    norm [delta; delta_only unfold_steps; primops];;
-    trytac implies_intros';;
-    dump "Initial goal";;
-    step_bind;;
-    step_bind;;
-    step_read_write;;
-    step_intro;;
-    step_extract_disjoint;;
-    step_read_write;;
-    step_eq_implies_intro;;
-    step_extract_disjoint;;
-    step_bind;;
-    step_read_write;;
-    step_intro;;
-    step_extract_disjoint;;
-    step_read_write;;
-    dump "See from here";;
-    step_eq_implies_intro;;
-    fail "End: double_increment_ok"
-  )
+  assert_by_tactic (h `contains` r /\ sel h r == n ==> t) solve
+
+// let rotate_ok (r1:addr) (r2:addr) (r3:addr) (h:heap) (i:t) (j:t) (k:t) =
+//   let c = Bind (Bind (Read r1) (fun n1 -> Bind (Read r2) (fun n2 -> Bind (Write r1 n2) (fun _ -> Write r2 n1)))) (fun _ -> Bind (Read r2) (fun n3 -> Bind (Read r3) (fun n4 -> Bind (Write r2 n4) (fun _ -> Write r3 n3)))) in
+//   let p = fun _ h -> (sel h r1 == j /\ sel h r2 == k /\ sel h r3 == i) in
+//   let t = (lift_wpsep (wpsep_command c)) p h in
+//   assert_by_tactic (h `contains` r1 /\ h `contains` r2 /\ h `contains` r3 /\ 
+//                     addr_of r1 <> addr_of r2 /\ addr_of r2 <> addr_of r3 /\ addr_of r1 <> addr_of r3 /\
+// 		    sel h r1 == i /\ sel h r2 == j /\ sel h r3 == k ==> t) solve
+
+let init_ok (h:heap) =
+  let c = Bind (Alloc) (fun (r1:addr) -> Bind (Write r1 7uL) (fun _ -> Return r1)) in
+  let p = fun r h -> sel h r == 7uL in
+  let t = (lift_wpsep (wpsep_command c)) p h in
+  assert_by_tactic t solve 
+
+let copy_ok (r1:addr) (r2:addr) (r3:addr) (h:heap) (i:t) (j:t) (k:t) =
+  let c = Bind (Read r1) (fun n1 -> Write r2 (n1)) in
+  let p = fun _ h -> (sel h r1 == i /\ sel h r2 == i /\ sel h r3 == k) in
+  let post = (lift_wpsep (wpsep_command c)) p h in
+  assert_by_tactic (h `contains` r1 /\ h `contains` r2 /\ h `contains` r3 /\ addr_of r1 <> addr_of r2 /\ addr_of r2 <> addr_of r3 /\ addr_of r1 <> addr_of r3 /\ sel h r1 == i /\ sel h r2 == j /\ sel h r3 == k ==> post) solve
